Canonical form lemma for type functions

CC/Subtype/Inversion.lean
@@ -13,6 +13,7 @@ import CC.Subcapt.Rename
 import CC.Subtype
 import CC.Subtype.Basic
 import CC.Subtype.Subst
+import CC.Subtype.TypeSubst
 
 namespace CC
 
@@ -53,7 +54,7 @@ lemma SubtypeP.tvar_inv :
   intro h
   apply SubtypeP.tvar_inv' <;> trivial
 
-def SubtypeP.fun_inv_motive (Γ : Ctx n m) (S1 S2 : PType n m) : Prop :=
+private def SubtypeP.fun_inv_motive (Γ : Ctx n m) (S1 S2 : PType n m) : Prop :=
   ∀ T U, 
     S2 = PType.arr T U ->
     SubtypeP Γ S1 S2 ->
@@ -136,3 +137,82 @@ theorem SubtypeP.fun_inv :
   (∃ T' U', P = PType.arr T' U' ∧ Subtype Γ T T' ∧ Subtype (Ctx.extend_var Γ T) U' U) := by
   intros
   apply SubtypeP.fun_inv' <;> aesop
+
+private def SubtypeP.tfun_inv_motive (Γ : Ctx n m) (S1 S2 : PType n m) : Prop :=
+  ∀ T U, 
+    S2 = PType.tarr T U ->
+    SubtypeP Γ S1 S2 ->
+    (∃ X, S1 = PType.tvar X) ∨ 
+    (∃ T' U', S1 = PType.tarr T' U' ∧ SubtypeP Γ T T' ∧ Subtype (Ctx.extend_tvar Γ T) U' U)
+
+lemma SubtypeP.tfun_inv' 
+  (h : SubtypeP Γ S1 S2) :
+  SubtypeP.tfun_inv_motive Γ S1 S2 := by
+  apply SubtypeP.rec
+    (motive_1 := fun Γ T1 T2 _ => True)
+    (motive_2 := fun Γ S1 S2 _ => SubtypeP.tfun_inv_motive Γ S1 S2)
+    <;> try (solve | trivial | intros; trivial | intros; unfold tfun_inv_motive; intros _ _ he; cases he)
+  case refl =>
+    intros; unfold tfun_inv_motive
+    intros
+    apply Or.inr
+    repeat apply Exists.intro
+    constructor
+    trivial
+    constructor
+    apply SubtypeP.refl
+    apply Subtype.refl
+  case trans =>
+    intros; unfold tfun_inv_motive at *
+    intros T U he h
+    rename_i h1 h2 ih1 ih2
+    subst_vars
+    have ih2' := ih2 _ _ rfl h2
+    cases ih2'
+    case inl ih =>
+      let ⟨X0, he0⟩ := ih
+      subst_vars
+      have h1' := SubtypeP.tvar_inv h1
+      aesop
+    case inr ih =>
+      let ⟨T', U', he, ih1, ih2⟩ := ih
+      subst_vars
+      have ih' := ih1 _ _ rfl h1
+      cases ih'
+      case inl => aesop
+      case inr ih' =>
+        let ⟨T'', U'', he', ih1', ih2'⟩ := ih'
+        subst_vars
+        apply Or.inr
+        repeat apply Exists.intro
+        constructor
+        trivial
+        constructor
+        apply SubtypeP.trans <;> trivial
+        apply Subtype.trans
+        · apply Subtype.narrow_tvar <;> trivial
+        · assumption
+  case tvar =>
+    intros; unfold tfun_inv_motive at *
+    intros T U he h
+    subst_vars
+    apply Or.inl
+    apply Exists.intro
+    rfl
+  case tarr =>
+    intros; unfold tfun_inv_motive at *
+    intros T U he h
+    subst_vars
+    apply Or.inr
+    repeat apply Exists.intro
+    constructor
+    rfl
+    cases he
+    constructor <;> trivial
+
+lemma SubtypeP.tfun_inv :
+  SubtypeP Γ P (PType.tarr T U) ->
+  (∃ X, P = PType.tvar X) ∨ 
+  (∃ T' U', P = PType.tarr T' U' ∧ SubtypeP Γ T T' ∧ Subtype (Ctx.extend_tvar Γ T) U' U) := by
+  intro h
+  apply SubtypeP.tfun_inv' <;> aesop
