CC/Narrowing.lean
@@ -14,6 +14,8 @@ import CC.Subtype
 import CC.Subtype.Rename
 import CC.Subtype.Basic
 import CC.Subst
+import CC.TypeMap
+import CC.Type.TypeSubst
 
 namespace CC
 
@@ -47,3 +49,29 @@ def TVarRename.narrowing_var :
   cases h
   constructor
   trivial
+
+def VarTypeMap.narrowing_tvar :
+  VarTypeMap (Ctx.extend_tvar Γ T) (Ctx.extend_tvar Γ T') TypeMap.id := by
+  unfold VarTypeMap
+  intros x T h
+  cases h
+  simp [CType.tsubst_id]
+  constructor; trivial
+
+def TVarSubst.narrowing_tvar (h : SubtypeP Γ T' T) :
+  TVarSubst (Ctx.extend_tvar Γ T) (Ctx.extend_tvar Γ T') TypeMap.id := by
+  unfold TVarSubst
+  intros X S h
+  cases h with
+  | here =>
+    simp [PType.tsubst_id]
+    simp [TypeMap.id]
+    apply SubtypeP.trans
+    apply SubtypeP.tvar
+    constructor
+    apply SubtypeP.weaken_tvar; trivial
+  | there_tvar hb =>
+    simp [PType.tsubst_id]
+    simp [TypeMap.id]
+    apply SubtypeP.tvar
+    constructor; trivial
